TouhouFormal/ECL.lean
@@ -17,6 +17,7 @@ import TouhouFormal.ECL.FloatFunction
 import TouhouFormal.ECL.Random
 import TouhouFormal.ECL.Movement
 import TouhouFormal.ECL.TimedMovement
+import TouhouFormal.ECL.OrbitMovement
 import TouhouFormal.ECL.EnemyState
 import TouhouFormal.ECL.Shooting
 import TouhouFormal.ECL.BulletPattern
